rustfrontend/Rusttypes.v
@@ -19,6 +19,8 @@ Inductive usekind : Type :=
 Inductive type : Type :=
 | Tunit: type                                    (**r the [unit] type *)
 | Tint: intsize -> signedness -> attr -> type       (**r integer types *)
+| Tlong : signedness -> attr -> type
+| Tfloat : floatsize -> attr -> type
 | Tfunction: typelist -> type -> calling_convention -> type    (**r function types *)
 | Tstruct: ident -> attr -> type                              (**r struct types  *)
 | Tunion: ident -> attr -> type                               (**r union types *)
@@ -37,6 +39,18 @@ Proof.
   decide equality.
   decide equality.
 Defined.
+
+Definition attr_of_type (ty: type) :=
+  match ty with
+  | Tunit => noattr
+  | Tint sz si a => a
+  | Tlong si a => a
+  | Tfloat sz a => a
+  | Tfunction args res cc => noattr
+  | Tstruct id a => a
+  | Tunion id a => a
+  end.
+
 
 (** Composite  *)
 
@@ -97,13 +111,425 @@ Record composite : Type := {
 
 Definition composite_env : Type := PTree.t composite.
 
-(** Access modes for members of structs or unions: either a plain field
-    or a bitfield *)
+(** ** Complete types *)
 
-Inductive bitfield : Type :=
-  | Full
-  | Bits (sz: intsize) (sg: signedness) (pos: Z) (width: Z).
+(** A type is complete if it fully describes an object.
+  All struct and union names appearing in the type must be defined,
+  unless they occur under a pointer or function type.  [void] and
+  function types are incomplete types. *)
 
+Fixpoint complete_type (env: composite_env) (t: type) : bool :=
+  match t with
+  | Tunit => false
+  | Tint _ _ _ => true
+  | Tlong _ _ => true
+  | Tfloat _ _ => true
+  | Tfunction _ _ _ => false
+  | Tstruct id _ | Tunion id _ =>
+      match env!id with Some co => true | None => false end
+  end.
+
+Definition complete_or_function_type (env: composite_env) (t: type) : bool :=
+  match t with
+  | Tfunction _ _ _ => true
+  | _ => complete_type env t
+  end.
+
+
+(** ** Alignment of a type *)
+
+(** Adjust the natural alignment [al] based on the attributes [a] attached
+  to the type.  If an "alignas" attribute is given, use it as alignment
+  in preference to [al]. *)
+
+Definition align_attr (a: attr) (al: Z) : Z :=
+  match attr_alignas a with
+  | Some l => two_p (Z.of_N l)
+  | None => al
+  end.
+
+Definition alignof (env: composite_env) (t: type) : Z :=
+  align_attr (attr_of_type t)
+   (match t with
+      | Tunit => 1
+      | Tint I8 _ _ => 1
+      | Tint I16 _ _ => 2
+      | Tint I32 _ _ => 4
+      | Tint IBool _ _ => 1
+      | Tlong _ _ => Archi.align_int64
+      | Tfloat F32 _ => 4
+      | Tfloat F64 _ => Archi.align_float64
+      | Tfunction _ _ _ => 1
+      | Tstruct id _ | Tunion id _ =>
+          match env!id with Some co => co_alignof co | None => 1 end
+    end).
+
+Remark align_attr_two_p:
+  forall al a,
+  (exists n, al = two_power_nat n) ->
+  (exists n, align_attr a al = two_power_nat n).
+Proof.
+  intros. unfold align_attr. destruct (attr_alignas a).
+  exists (N.to_nat n). rewrite two_power_nat_two_p. rewrite N_nat_Z. auto.
+  auto.
+Qed.
+
+Lemma alignof_two_p:
+  forall env t, exists n, alignof env t = two_power_nat n.
+Proof.
+  induction t; apply align_attr_two_p; simpl.
+  exists 0%nat; auto.
+  destruct i.
+    exists 0%nat; auto.
+    exists 1%nat; auto.
+    exists 2%nat; auto.
+    exists 0%nat; auto.
+    unfold Archi.align_int64. destruct Archi.ptr64; ((exists 2%nat; reflexivity) || (exists 3%nat; reflexivity)).
+  destruct f.
+    exists 2%nat; auto.
+    unfold Archi.align_float64. destruct Archi.ptr64; ((exists 2%nat; reflexivity) || (exists 3%nat; reflexivity)).
+  exists 0%nat; auto.
+  destruct (env!i). apply co_alignof_two_p. exists 0%nat; auto.
+  destruct (env!i). apply co_alignof_two_p. exists 0%nat; auto.
+Qed.
+
+Lemma alignof_pos:
+  forall env t, alignof env t > 0.
+Proof.
+  intros. destruct (alignof_two_p env t) as [n EQ]. rewrite EQ. apply two_power_nat_pos.
+Qed.
+
+(** Size of a type  *)
+
+Definition sizeof (env: composite_env) (t: type) : Z :=
+  match t with
+  | Tunit => 1
+  | Tint I8 _ _ => 1
+  | Tint I16 _ _ => 2
+  | Tint I32 _ _
+  | Tfloat F32 _ => 4
+  | Tint IBool _ _ => 1
+  | Tlong _ _
+  | Tfloat F64 _ => 8
+  | Tfunction _ _ _ => 1
+  | Tstruct id _
+  | Tunion id _ =>
+      match env!id with
+      | Some co => co_sizeof co
+      | None => 0
+      end                    
+  end.
+
+Lemma sizeof_pos:
+  forall env t, sizeof env t >= 0.
+Proof.
+  induction t; simpl.
+- lia.
+- destruct i; lia.
+- lia.
+- destruct f; lia.
+- destruct Archi.ptr64; lia.
+- destruct (env!i). apply co_sizeof_pos. lia.
+- destruct (env!i). apply co_sizeof_pos. lia.
+Qed.
+
+Definition alignof_blockcopy (env: composite_env) (t: type) : Z :=
+  match t with
+  | Tunit => 1
+  | Tint I8 _ _ => 1
+  | Tint I16 _ _ => 2
+  | Tint I32 _ _
+  | Tfloat F32 _ => 4
+  | Tlong _ _
+  | Tfloat F64 _ => 8
+  | Tint IBool _ _ => 1
+  | Tfunction _ _ _ => 1
+  | Tstruct id _
+  | Tunion id _ =>
+      match env!id with
+      | Some co => Z.min 8 (co_alignof co)
+      | None => 1
+      end
+  end.
+
+
+
+(** ** Layout of struct fields *)
+
+Section LAYOUT.
+
+Variable env: composite_env.
+
+Definition bitalignof (t: type) := alignof env t * 8.
+
+Definition bitsizeof  (t: type) := sizeof env t * 8.
+
+Definition bitalignof_intsize (sz: intsize) : Z :=
+  match sz with
+  | I8 | IBool => 8
+  | I16 => 16
+  | I32 => 32
+  end.
+
+Definition next_field (pos: Z) (m: member) : Z :=
+  match m with
+  | Member_plain _ t =>
+      align pos (bitalignof t) + bitsizeof t
+  end.
+
+Definition layout_field (pos: Z) (m: member) : res (Z * bitfield) :=
+  match m with
+  | Member_plain _ t =>
+      OK (align pos (bitalignof t) / 8, Full)
+  end.
+
+(** Some properties *)
+
+Lemma bitalignof_intsize_pos:
+  forall sz, bitalignof_intsize sz > 0.
+Proof.
+  destruct sz; simpl; lia.
+Qed.
+
+Lemma next_field_incr:
+  forall pos m, pos <= next_field pos m.
+Proof.
+  intros. unfold next_field. destruct m.
+- set (al := bitalignof t).
+  assert (A: al > 0).
+  { unfold al, bitalignof. generalize (alignof_pos env t). lia. }
+  assert (pos <= align pos al) by (apply align_le; auto).
+  assert (bitsizeof t >= 0).
+  { unfold bitsizeof. generalize (sizeof_pos env t). lia. } 
+  lia.
+Qed.
+
+Definition layout_start (p: Z) (bf: bitfield) :=
+  p * 8 + match bf with Full => 0 | Bits sz sg pos w => pos end.
+
+Definition layout_width (t: type) (bf: bitfield) :=
+  match bf with Full => bitsizeof t | Bits sz sg pos w => w end.
+
+Lemma layout_field_range: forall pos m ofs bf,
+  layout_field pos m = OK (ofs, bf) ->
+  pos <= layout_start ofs bf 
+  /\ layout_start ofs bf + layout_width (type_member m) bf <= next_field pos m.
+Proof.
+  intros until bf; intros L. unfold layout_start, layout_width. destruct m; simpl in L.
+- inv L. simpl.
+  set (al := bitalignof t).
+  set (q := align pos al).
+  assert (A: al > 0).
+  { unfold al, bitalignof. generalize (alignof_pos env t). lia. }
+  assert (B: pos <= q) by (apply align_le; auto).
+  assert (C: (al | q)) by (apply align_divides; auto).
+  assert (D: (8 | q)). 
+  { apply Z.divide_transitive with al; auto. apply Z.divide_factor_r. }
+  assert (E: q / 8 * 8 = q).
+  { destruct D as (n & E). rewrite E. rewrite Z.div_mul by lia. auto. }
+  rewrite E. lia.
+Qed.
+
+Definition layout_alignment (t: type) (bf: bitfield) :=
+  match bf with
+  | Full => alignof env t
+  | Bits sz _ _ _ => bitalignof_intsize sz / 8
+  end.
+
+Lemma layout_field_alignment: forall pos m ofs bf,
+  layout_field pos m = OK (ofs, bf) ->
+  (layout_alignment (type_member m) bf | ofs).
+Proof.
+  intros until bf; intros L. destruct m; simpl in L.
+- inv L; simpl. 
+  set (q := align pos (bitalignof t)).
+  assert (A: (bitalignof t | q)).
+  { apply align_divides. unfold bitalignof. generalize (alignof_pos env t). lia. }
+  destruct A as [n E]. exists n. rewrite E. unfold bitalignof. rewrite Z.mul_assoc, Z.div_mul by lia. auto.
+Qed.
+
+End LAYOUT.
+
+
+(** ** Size and alignment for composite definitions *)
+
+(** The alignment for a structure or union is the max of the alignment
+  of its members.  Padding bitfields are ignored. *)
+
+Fixpoint alignof_composite (env: composite_env) (ms: members) : Z :=
+  match ms with
+  | nil => 1
+  | m :: ms => 
+     if member_is_padding m
+     then alignof_composite env ms
+     else Z.max (alignof env (type_member m)) (alignof_composite env ms)
+  end.
+
+(** The size of a structure corresponds to its layout: fields are
+  laid out consecutively, and padding is inserted to align
+  each field to the alignment for its type.  Bitfields are packed
+  as described above. *)
+
+Fixpoint bitsizeof_struct (env: composite_env) (cur: Z) (ms: members) : Z :=
+  match ms with
+  | nil => cur
+  | m :: ms => bitsizeof_struct env (next_field env cur m) ms
+  end.
+
+Definition bytes_of_bits (n: Z) := (n + 7) / 8.
+
+Definition sizeof_struct (env: composite_env) (m: members) : Z :=
+  bytes_of_bits (bitsizeof_struct env 0 m).
+
+(** The size of an union is the max of the sizes of its members. *)
+
+Fixpoint sizeof_union (env: composite_env) (ms: members) : Z :=
+  match ms with
+  | nil => 0
+  | m :: ms => Z.max (sizeof env (type_member m)) (sizeof_union env ms)
+  end.
+
+
+(** Some properties *)
+
+Lemma alignof_composite_two_p:
+  forall env m, exists n, alignof_composite env m = two_power_nat n.
+Proof.
+  induction m; simpl.
+- exists 0%nat; auto.
+- destruct (member_is_padding a); auto.
+  apply Z.max_case; auto. apply alignof_two_p.
+Qed.
+
+Lemma alignof_composite_pos:
+  forall env m a, align_attr a (alignof_composite env m) > 0.
+Proof.
+  intros.
+  exploit align_attr_two_p. apply (alignof_composite_two_p env m).
+  instantiate (1 := a). intros [n EQ].
+  rewrite EQ; apply two_power_nat_pos.
+Qed.
+
+Lemma bitsizeof_struct_incr:
+  forall env m cur, cur <= bitsizeof_struct env cur m.
+Proof.
+  induction m; simpl; intros.
+- lia.
+- apply Z.le_trans with (next_field env cur a).
+  apply next_field_incr. apply IHm.
+Qed.
+
+Lemma sizeof_union_pos:
+  forall env m, 0 <= sizeof_union env m.
+Proof.
+  induction m; simpl; extlia.
+Qed.
+
+(** Type ranks *)
+
+(** The rank of a type is a nonnegative integer that measures the direct nesting
+  of arrays, struct and union types.  It does not take into account indirect
+  nesting such as a struct type that appears under a pointer or function type.
+  Type ranks ensure that type expressions (ignoring pointer and function types)
+  have an inductive structure. *)
+
+Fixpoint rank_type (ce: composite_env) (t: type) : nat :=
+  match t with
+  | Tstruct id _ | Tunion id _ =>
+      match ce!id with
+      | None => O
+      | Some co => S (co_rank co)
+      end
+  | _ => O
+  end.
+
+Fixpoint rank_members (ce: composite_env) (m: members) : nat :=
+  match m with
+  | nil => 0%nat
+  | Member_plain _ t :: m => Init.Nat.max (rank_type ce t) (rank_members ce m)
+  end.
+
+
+(** * Construction of the composite environment *)
+
+Definition sizeof_composite (env: composite_env) (su: struct_or_union) (m: members) : Z :=
+  match su with
+  | Struct => sizeof_struct env m
+  | Union  => sizeof_union env m
+  end.
+
+Lemma sizeof_composite_pos:
+  forall env su m, 0 <= sizeof_composite env su m.
+Proof.
+  intros. destruct su; simpl.
+- unfold sizeof_struct, bytes_of_bits.
+  assert (0 <= bitsizeof_struct env 0 m) by apply bitsizeof_struct_incr.
+  change 0 with (0 / 8) at 1. apply Z.div_le_mono; lia.
+- apply sizeof_union_pos.
+Qed.
+
+Fixpoint complete_members (env: composite_env) (ms: members) : bool :=
+  match ms with
+  | nil => true
+  | m :: ms => complete_type env (type_member m) && complete_members env ms
+  end.
+
+Lemma complete_member:
+  forall env m ms,
+  In m ms -> complete_members env ms = true -> complete_type env (type_member m) = true.
+Proof.
+  induction ms as [|m1 ms]; simpl; intuition auto.
+  InvBooleans; inv H1; auto.
+  InvBooleans; eauto.
+Qed.
+
+Program Definition composite_of_def
+     (env: composite_env) (id: ident) (su: struct_or_union) (m: members) (a: attr)
+     : res composite :=
+  match env!id, complete_members env m return _ with
+  | Some _, _ =>
+      Error (MSG "Multiple definitions of struct or union " :: CTX id :: nil)
+  | None, false =>
+      Error (MSG "Incomplete struct or union " :: CTX id :: nil)
+  | None, true =>
+      let al := align_attr a (alignof_composite env m) in
+      OK {| co_su := su;
+            co_members := m;
+            co_attr := a;
+            co_sizeof := align (sizeof_composite env su m) al;
+            co_alignof := al;
+            co_rank := rank_members env m;
+            co_sizeof_pos := _;
+            co_alignof_two_p := _;
+            co_sizeof_alignof := _ |}
+  end.
+Next Obligation.
+  apply Z.le_ge. eapply Z.le_trans. eapply sizeof_composite_pos.
+  apply align_le; apply alignof_composite_pos.
+Defined.
+Next Obligation.
+  apply align_attr_two_p. apply alignof_composite_two_p.
+Defined.
+Next Obligation.
+  apply align_divides. apply alignof_composite_pos.
+Defined.
+
+(** The composite environment for a program is obtained by entering
+  its composite definitions in sequence.  The definitions are assumed
+  to be listed in dependency order: the definition of a composite
+  must precede all uses of this composite, unless the use is under
+  a pointer or function type. *)
+
+Fixpoint add_composite_definitions (env: composite_env) (defs: list composite_definition) : res composite_env :=
+  match defs with
+  | nil => OK env
+  | Composite id su m a :: defs =>
+      do co <- composite_of_def env id su m a;
+      add_composite_definitions (PTree.set id co env) defs
+  end.
+
+Definition build_composite_env (defs: list composite_definition) :=
+  add_composite_definitions (PTree.empty _) defs.
 
 Section PROGRAMS.
 
